src/prop/PFConsistentStrong.v
@@ -1,0 +1,212 @@
+Require Import Omega.
+Require Import Bool.
+Require Import RelationClasses.
+
+From sflib Require Import sflib.
+From Paco Require Import paco.
+
+From PromisingLib Require Import Axioms.
+From PromisingLib Require Import Basic.
+From PromisingLib Require Import DataStructure.
+From PromisingLib Require Import DenseOrder.
+From PromisingLib Require Import Language.
+From PromisingLib Require Import Loc.
+
+Require Import Event.
+Require Import Time.
+Require Import View.
+Require Import Cell.
+Require Import Memory.
+Require Import TView.
+Require Import Local.
+Require Import Thread.
+Require Import Pred.
+Require Import MemoryMerge.
+Require Import PromiseConsistent.
+Require Import PFConsistent.
+Require Import ReorderPromises2.
+Require Import MemoryProps.
+
+Set Implicit Arguments.
+
+
+Definition pf_consistent_strong lang (e0:Thread.t lang): Prop :=
+  forall mem1 sc1
+         (CAP: Memory.cap e0.(Thread.memory) mem1),
+  exists e1,
+    (<<STEPS0: rtc (tau (@pred_step is_cancel lang)) (Thread.mk _ e0.(Thread.state) e0.(Thread.local) sc1 mem1) e1>>) /\
+    (<<NORESERVE: no_reserves e1.(Thread.local).(Local.promises)>>) /\
+    exists e2,
+      (<<STEPS1: rtc (tau (@pred_step ((promise_free /1\ (fun e => ~ is_cancel e)) /1\ no_sc) lang)) e1 e2>>) /\
+      (__guard__((exists st',
+                     (<<LOCAL: Local.failure_step e2.(Thread.local)>>) /\
+                     (<<FAILURE: Language.step lang ProgramEvent.failure (@Thread.state lang e2) st'>>)) \/
+                 (<<PROMISES: e2.(Thread.local).(Local.promises) = Memory.bot>>))).
+
+Lemma step_promise_consistent
+      lang pf e th1 th2
+      (STEP: @Thread.step lang pf e th1 th2)
+      (CONS: Local.promise_consistent th2.(Thread.local))
+      (WF1: Local.wf th1.(Thread.local) th1.(Thread.memory))
+      (SC1: Memory.closed_timemap th1.(Thread.sc) th1.(Thread.memory))
+      (MEM1: Memory.closed th1.(Thread.memory)):
+  Local.promise_consistent th1.(Thread.local).
+Proof.
+  inv STEP; [inv STEP0|inv STEP0; inv LOCAL]; ss.
+  - eapply promise_step_promise_consistent; eauto.
+  - eapply read_step_promise_consistent; eauto.
+  - eapply write_step_promise_consistent; eauto.
+  - eapply read_step_promise_consistent; eauto.
+    eapply write_step_promise_consistent; eauto.
+  - eapply fence_step_promise_consistent; eauto.
+  - eapply fence_step_promise_consistent; eauto.
+Qed.
+
+Lemma pf_consistent_pf_consistent_strong lang (th: Thread.t lang)
+      (WF: Local.wf th.(Thread.local) th.(Thread.memory))
+      (MEM: Memory.closed th.(Thread.memory))
+      (CONSISTENT: pf_consistent th)
+  :
+    pf_consistent_strong th.
+Proof.
+  assert (INHABITED: Memory.inhabited th.(Thread.memory)).
+  { inv MEM. auto. }
+  ii. exploit Memory.max_concrete_timemap_exists; eauto. intros MAX. des.
+  ii. exploit Memory.max_concrete_timemap_exists.
+  { eapply le_inhabited; eauto. eapply Memory.cap_le; eauto. refl. }
+  i. des. exploit CONSISTENT; eauto. i.
+
+  assert (exists e2,
+             (<<STEPS: rtc (tau (Thread.step true))
+                           (Thread.mk _ (Thread.state th) (Thread.local th)
+                                      tm0 mem1) e2 >>) /\
+             (<<NORESERVES: no_reserves e2.(Thread.local).(Local.promises)>>) /\
+             (__guard__ ((exists e3, (<< FAILURE: Thread.step true ThreadEvent.failure e2 e3 >>)) \/
+                         (<<PROMISES: Local.promises (Thread.local e2) = Memory.bot >>)))).
+  { des.
+    - exploit Thread.rtc_tau_step_future.
+      + eapply rtc_implies; [|apply STEPS].
+        i. inv PR. econs; eauto. econs; eauto.
+      + ss. eapply Local.cap_wf; eauto.
+      + ss. eapply Memory.max_concrete_timemap_closed; eauto.
+      + ss. eapply Memory.cap_closed; eauto.
+      + i. des.
+        destruct e2. destruct local. inv WF2. ss.
+        exploit reserves_cancelable; eauto. i. des.
+        esplits.
+        * etrans.
+          { eapply STEPS. }
+          { eapply rtc_implies; [|apply STEPS0].
+            i. inv PR. inv TSTEP. inv STEP.
+            unfold is_cancel in SAT. des_ifs.
+            inv STEP0; inv STEP.
+            - econs; eauto. econs; eauto. econs; eauto.
+            - inv LOCAL. }
+        * ss.
+        * left. inv FAILURE; inv STEP. inv LOCAL. inv LOCAL0.
+          exists (Thread.mk _ st2 (Local.mk tview proms1) sc2 mem0).
+          ss. econs 2. econs; eauto. econs; eauto. econs; eauto.
+          eapply nacancels_promises_decrease in STEPS0; auto. ss.
+          ii. eapply CONSISTENT0; eauto.
+    - unguard. esplits; eauto. rewrite PROMISES. ii.
+      rewrite Memory.bot_get in GET. clarify. }
+
+  clear x. des.
+  eapply pf_step_promise_free_step_rtc in STEPS.
+  eapply pf_steps_cancels_not_cancels in STEPS; cycle 1.
+  { ss. eapply Local.cap_wf; eauto. }
+  { ss. eapply Memory.cap_closed; eauto. }
+  { ss. eapply Memory.max_concrete_timemap_closed; eauto. } des.
+
+  exploit Thread.rtc_tau_step_future.
+  { eapply thread_steps_pred_steps. eapply STEPS1. }
+  { ss. eapply Local.cap_wf; eauto. }
+  { ss. eapply Memory.max_concrete_timemap_closed; eauto. }
+  { ss. eapply Memory.cap_closed; eauto. }
+  i. des. ss.
+
+  destruct th1. exploit no_sc_any_sc_rtc; try apply STEPS1; ss.
+  { i. unfold is_cancel in PR. des_ifs. }
+  i. des. instantiate (1:=sc1) in STEP. clear STEPS1.
+
+  eexists. splits.
+  { eapply STEP. }
+  { ss. ii. clarify.
+    eapply steps_not_cancel_reserves_same in STEPS2; eauto.
+    unguard. des.
+    - eapply NORESERVES; eauto.
+    - rewrite PROMISES in *. erewrite Memory.bot_get in STEPS2. clarify. }
+
+  eapply hold_or_not with (Q := no_sc) in STEPS2. des.
+
+  - destruct e2. ss.
+    exploit no_sc_any_sc_rtc; try eapply HOLD; eauto.
+    { ss. i. des. auto. } i. des.
+    esplits.
+    + eapply pred_step_rtc_mon; try eapply STEP0. i. ss.
+    + ss. unguard. des.
+      * left. ss. inv FAILURE; inv STEP1. inv LOCAL. eauto.
+      * right. esplits; eauto.
+
+  - exploit Thread.rtc_tau_step_future.
+    { eapply thread_steps_pred_steps. eapply STEPS0. }
+    { ss. }
+    { ss. }
+    { ss. } i. des.
+    inv STEP0.
+    exploit Thread.step_future; eauto. i. des.
+
+    assert (PROMS: Local.promise_consistent e3.(Thread.local)).
+    { eapply rtc_tau_step_promise_consistent.
+      - eapply thread_steps_pred_steps. eapply STEPS1.
+      - unguard. des.
+        + inv FAILURE; inv STEP0. inv LOCAL. inv LOCAL0. ss.
+        + ii. rewrite PROMISES in PROMISE.
+          rewrite Memory.bot_get in PROMISE. clarify.
+      - eauto.
+      - eauto.
+      - eauto. }
+
+    assert (NOPROMISE: e2'.(Thread.local).(Local.promises) = Memory.bot).
+    { apply Memory.ext. i. rewrite Memory.bot_get.
+      destruct (Memory.get loc ts (Local.promises (Thread.local e2')))
+        as [[from [val released|]]|] eqn:GET; auto; cycle 1.
+      - exfalso.
+        eapply step_not_cancel_reserves_same in GET; cycle 1.
+        + econs.
+          * econs; eauto.
+          * instantiate (1:=promise_free /1\ (fun e => ~ is_cancel e)). ss.
+        + ss.
+        + des. eapply steps_not_cancel_reserves_same in GET; eauto.
+          des. eapply NORESERVES; eauto.
+      - exfalso.
+        exploit pf_step_rtc_promises_decrease.
+        { eapply STEPS0. }
+        { i. ss. des. auto. }
+        { econs; eauto. } ss. i.
+        exploit pf_step_rtc_promises_decrease.
+        { eapply STEP. }
+        { i. unfold is_cancel in *. des_ifs. }
+        { ss. eauto. }
+        ss. i. inv x2.
+        ss. unfold no_sc in BREAKQ. des_ifs; try by (exfalso; eauto).
+        + des; clarify. apply NNPP in BREAKQ.
+          inv STEP1; inv STEP0. ss. inv LOCAL. inv LOCAL0. ss.
+          eapply PROMS in GET. ss. des_ifs. ss.
+          hexploit max_concrete_timemap_get; eauto.
+          * inv WF. eapply Memory.cap_le; eauto.
+          * i. eapply Time.lt_strorder. eapply TimeFacts.lt_le_lt; eauto.
+        + inv STEP1; inv STEP0. ss. inv LOCAL. inv LOCAL0. ss.
+          eapply PROMS in GET. ss. des_ifs. ss.
+          hexploit max_concrete_timemap_get; eauto.
+          * inv WF. eapply Memory.cap_le; eauto.
+          * i. eapply Time.lt_strorder. eapply TimeFacts.lt_le_lt; eauto.
+    }
+
+    destruct e2'. destruct local. ss.
+    eapply no_sc_any_sc_rtc in STEPS0; ss; cycle 1.
+    { i. des; ss. } des.
+    esplits.
+    * eapply pred_step_rtc_mon; eauto. i. ss.
+    * unguard. ss. eauto.
+Qed.
